CoqOfRust/examples/default/examples/ink_contracts/multisig.v
@@ -259,40 +259,6 @@ Section Impl_core_marker_Copy_for_multisig_AccountId_t.
 End Impl_core_marker_Copy_for_multisig_AccountId_t.
 End Impl_core_marker_Copy_for_multisig_AccountId_t.
 
-Module  Impl_core_cmp_Ord_for_multisig_AccountId_t.
-Section Impl_core_cmp_Ord_for_multisig_AccountId_t.
-  Ltac Self := exact multisig.AccountId.t.
-  
-  (*
-  Ord
-  *)
-  Definition cmp
-      (self : ref ltac:(Self))
-      (other : ref multisig.AccountId.t)
-      : M core.cmp.Ordering.t :=
-    let* self : M.Val (ref ltac:(Self)) := M.alloc self in
-    let* other : M.Val (ref multisig.AccountId.t) := M.alloc other in
-    let* α0 : ref multisig.AccountId.t := M.read self in
-    let* α1 : ref multisig.AccountId.t := M.read other in
-    M.call
-      ((core.cmp.Ord.cmp (Self := u128.t) (Trait := ltac:(refine _)))
-        (borrow (deref α0).["0"])
-        (borrow (deref α1).["0"])).
-  
-  Global Instance AssociatedFunction_cmp :
-    Notations.DoubleColon ltac:(Self) "cmp" := {
-    Notations.double_colon := cmp;
-  }.
-  
-  Global Instance ℐ : core.cmp.Ord.Required.Trait ltac:(Self) := {
-    core.cmp.Ord.cmp := cmp;
-    core.cmp.Ord.max := Datatypes.None;
-    core.cmp.Ord.min := Datatypes.None;
-    core.cmp.Ord.clamp := Datatypes.None;
-  }.
-End Impl_core_cmp_Ord_for_multisig_AccountId_t.
-End Impl_core_cmp_Ord_for_multisig_AccountId_t.
-
 Module  Impl_core_marker_StructuralPartialEq_for_multisig_AccountId_t.
 Section Impl_core_marker_StructuralPartialEq_for_multisig_AccountId_t.
   Ltac Self := exact multisig.AccountId.t.
@@ -334,6 +300,113 @@ Section Impl_core_cmp_PartialEq_for_multisig_AccountId_t.
   }.
 End Impl_core_cmp_PartialEq_for_multisig_AccountId_t.
 End Impl_core_cmp_PartialEq_for_multisig_AccountId_t.
+
+Module  Impl_core_marker_StructuralEq_for_multisig_AccountId_t.
+Section Impl_core_marker_StructuralEq_for_multisig_AccountId_t.
+  Ltac Self := exact multisig.AccountId.t.
+  
+  Global Instance ℐ : core.marker.StructuralEq.Trait ltac:(Self) := {
+  }.
+End Impl_core_marker_StructuralEq_for_multisig_AccountId_t.
+End Impl_core_marker_StructuralEq_for_multisig_AccountId_t.
+
+Module  Impl_core_cmp_Eq_for_multisig_AccountId_t.
+Section Impl_core_cmp_Eq_for_multisig_AccountId_t.
+  Ltac Self := exact multisig.AccountId.t.
+  
+  (*
+  Eq
+  *)
+  Definition assert_receiver_is_total_eq (self : ref ltac:(Self)) : M unit :=
+    let* self : M.Val (ref ltac:(Self)) := M.alloc self in
+    let* _ : M.Val unit := M.alloc tt in
+    let* α0 : M.Val unit := M.alloc tt in
+    M.read α0.
+  
+  Global Instance AssociatedFunction_assert_receiver_is_total_eq :
+    Notations.DoubleColon ltac:(Self) "assert_receiver_is_total_eq" := {
+    Notations.double_colon := assert_receiver_is_total_eq;
+  }.
+  
+  Global Instance ℐ : core.cmp.Eq.Required.Trait ltac:(Self) := {
+    core.cmp.Eq.assert_receiver_is_total_eq :=
+      Datatypes.Some assert_receiver_is_total_eq;
+  }.
+End Impl_core_cmp_Eq_for_multisig_AccountId_t.
+End Impl_core_cmp_Eq_for_multisig_AccountId_t.
+
+Module  Impl_core_cmp_PartialOrd_for_multisig_AccountId_t.
+Section Impl_core_cmp_PartialOrd_for_multisig_AccountId_t.
+  Ltac Self := exact multisig.AccountId.t.
+  
+  (*
+  PartialOrd
+  *)
+  Definition partial_cmp
+      (self : ref ltac:(Self))
+      (other : ref multisig.AccountId.t)
+      : M (core.option.Option.t core.cmp.Ordering.t) :=
+    let* self : M.Val (ref ltac:(Self)) := M.alloc self in
+    let* other : M.Val (ref multisig.AccountId.t) := M.alloc other in
+    let* α0 : ref multisig.AccountId.t := M.read self in
+    let* α1 : ref multisig.AccountId.t := M.read other in
+    M.call
+      ((core.cmp.PartialOrd.partial_cmp
+          (Self := u128.t)
+          (Trait := ltac:(refine _)))
+        (borrow (deref α0).["0"])
+        (borrow (deref α1).["0"])).
+  
+  Global Instance AssociatedFunction_partial_cmp :
+    Notations.DoubleColon ltac:(Self) "partial_cmp" := {
+    Notations.double_colon := partial_cmp;
+  }.
+  
+  Global Instance ℐ :
+    core.cmp.PartialOrd.Required.Trait ltac:(Self)
+      (Rhs := core.cmp.PartialOrd.Default.Rhs ltac:(Self)) := {
+    core.cmp.PartialOrd.partial_cmp := partial_cmp;
+    core.cmp.PartialOrd.lt := Datatypes.None;
+    core.cmp.PartialOrd.le := Datatypes.None;
+    core.cmp.PartialOrd.gt := Datatypes.None;
+    core.cmp.PartialOrd.ge := Datatypes.None;
+  }.
+End Impl_core_cmp_PartialOrd_for_multisig_AccountId_t.
+End Impl_core_cmp_PartialOrd_for_multisig_AccountId_t.
+
+Module  Impl_core_cmp_Ord_for_multisig_AccountId_t.
+Section Impl_core_cmp_Ord_for_multisig_AccountId_t.
+  Ltac Self := exact multisig.AccountId.t.
+  
+  (*
+  Ord
+  *)
+  Definition cmp
+      (self : ref ltac:(Self))
+      (other : ref multisig.AccountId.t)
+      : M core.cmp.Ordering.t :=
+    let* self : M.Val (ref ltac:(Self)) := M.alloc self in
+    let* other : M.Val (ref multisig.AccountId.t) := M.alloc other in
+    let* α0 : ref multisig.AccountId.t := M.read self in
+    let* α1 : ref multisig.AccountId.t := M.read other in
+    M.call
+      ((core.cmp.Ord.cmp (Self := u128.t) (Trait := ltac:(refine _)))
+        (borrow (deref α0).["0"])
+        (borrow (deref α1).["0"])).
+  
+  Global Instance AssociatedFunction_cmp :
+    Notations.DoubleColon ltac:(Self) "cmp" := {
+    Notations.double_colon := cmp;
+  }.
+  
+  Global Instance ℐ : core.cmp.Ord.Required.Trait ltac:(Self) := {
+    core.cmp.Ord.cmp := cmp;
+    core.cmp.Ord.max := Datatypes.None;
+    core.cmp.Ord.min := Datatypes.None;
+    core.cmp.Ord.clamp := Datatypes.None;
+  }.
+End Impl_core_cmp_Ord_for_multisig_AccountId_t.
+End Impl_core_cmp_Ord_for_multisig_AccountId_t.
 
 Module  Impl_core_fmt_Debug_for_multisig_AccountId_t.
 Section Impl_core_fmt_Debug_for_multisig_AccountId_t.
@@ -385,81 +458,6 @@ Section Env.
   }.
 End Env.
 End Env.
-
-Module  Impl_multisig_Env_t.
-Section Impl_multisig_Env_t.
-  Ltac Self := exact multisig.Env.t.
-  
-  (*
-      fn caller(&self) -> AccountId {
-          self.caller
-      }
-  *)
-  Definition caller (self : ref ltac:(Self)) : M multisig.AccountId.t :=
-    let* self : M.Val (ref ltac:(Self)) := M.alloc self in
-    let* α0 : ref multisig.Env.t := M.read self in
-    M.read (deref α0).["caller"].
-  
-  Global Instance AssociatedFunction_caller :
-    Notations.DoubleColon ltac:(Self) "caller" := {
-    Notations.double_colon := caller;
-  }.
-  
-  (*
-      fn emit_event(&self, _event: Event) {
-          unimplemented!()
-      }
-  *)
-  Definition emit_event
-      (self : ref ltac:(Self))
-      (_event : multisig.Event.t)
-      : M unit :=
-    let* self : M.Val (ref ltac:(Self)) := M.alloc self in
-    let* _event : M.Val multisig.Event.t := M.alloc _event in
-    let* α0 : ref str.t := M.read (mk_str "not implemented") in
-    let* α1 : never.t := M.call (core.panicking.panic α0) in
-    never_to_any α1.
-  
-  Global Instance AssociatedFunction_emit_event :
-    Notations.DoubleColon ltac:(Self) "emit_event" := {
-    Notations.double_colon := emit_event;
-  }.
-  
-  (*
-      fn transferred_value(&self) -> Balance {
-          unimplemented!()
-      }
-  *)
-  Definition transferred_value
-      (self : ref ltac:(Self))
-      : M ltac:(multisig.Balance) :=
-    let* self : M.Val (ref ltac:(Self)) := M.alloc self in
-    let* α0 : ref str.t := M.read (mk_str "not implemented") in
-    let* α1 : never.t := M.call (core.panicking.panic α0) in
-    never_to_any α1.
-  
-  Global Instance AssociatedFunction_transferred_value :
-    Notations.DoubleColon ltac:(Self) "transferred_value" := {
-    Notations.double_colon := transferred_value;
-  }.
-  
-  (*
-      fn account_id(&self) -> AccountId {
-          unimplemented!()
-      }
-  *)
-  Definition account_id (self : ref ltac:(Self)) : M multisig.AccountId.t :=
-    let* self : M.Val (ref ltac:(Self)) := M.alloc self in
-    let* α0 : ref str.t := M.read (mk_str "not implemented") in
-    let* α1 : never.t := M.call (core.panicking.panic α0) in
-    never_to_any α1.
-  
-  Global Instance AssociatedFunction_account_id :
-    Notations.DoubleColon ltac:(Self) "account_id" := {
-    Notations.double_colon := account_id;
-  }.
-End Impl_multisig_Env_t.
-End Impl_multisig_Env_t.
 
 Definition MAX_OWNERS : u32.t := M.run (M.alloc (Integer.of_Z 50)).
 
@@ -647,15 +645,6 @@ Module Error.
   | TransactionFailed.
 End Error.
 
-Module  Impl_core_marker_Copy_for_multisig_Error_t.
-Section Impl_core_marker_Copy_for_multisig_Error_t.
-  Ltac Self := exact multisig.Error.t.
-  
-  Global Instance ℐ : core.marker.Copy.Trait ltac:(Self) := {
-  }.
-End Impl_core_marker_Copy_for_multisig_Error_t.
-End Impl_core_marker_Copy_for_multisig_Error_t.
-
 Module  Impl_core_clone_Clone_for_multisig_Error_t.
 Section Impl_core_clone_Clone_for_multisig_Error_t.
   Ltac Self := exact multisig.Error.t.
@@ -679,6 +668,15 @@ Section Impl_core_clone_Clone_for_multisig_Error_t.
   }.
 End Impl_core_clone_Clone_for_multisig_Error_t.
 End Impl_core_clone_Clone_for_multisig_Error_t.
+
+Module  Impl_core_marker_Copy_for_multisig_Error_t.
+Section Impl_core_marker_Copy_for_multisig_Error_t.
+  Ltac Self := exact multisig.Error.t.
+  
+  Global Instance ℐ : core.marker.Copy.Trait ltac:(Self) := {
+  }.
+End Impl_core_marker_Copy_for_multisig_Error_t.
+End Impl_core_marker_Copy_for_multisig_Error_t.
 
 Module  Impl_core_fmt_Debug_for_multisig_Error_t.
 Section Impl_core_fmt_Debug_for_multisig_Error_t.
@@ -1021,6 +1019,81 @@ Module Event.
   | OwnerRemoval (_ : multisig.OwnerRemoval.t)
   | RequirementChange (_ : multisig.RequirementChange.t).
 End Event.
+
+Module  Impl_multisig_Env_t.
+Section Impl_multisig_Env_t.
+  Ltac Self := exact multisig.Env.t.
+  
+  (*
+      fn caller(&self) -> AccountId {
+          self.caller
+      }
+  *)
+  Definition caller (self : ref ltac:(Self)) : M multisig.AccountId.t :=
+    let* self : M.Val (ref ltac:(Self)) := M.alloc self in
+    let* α0 : ref multisig.Env.t := M.read self in
+    M.read (deref α0).["caller"].
+  
+  Global Instance AssociatedFunction_caller :
+    Notations.DoubleColon ltac:(Self) "caller" := {
+    Notations.double_colon := caller;
+  }.
+  
+  (*
+      fn emit_event(&self, _event: Event) {
+          unimplemented!()
+      }
+  *)
+  Definition emit_event
+      (self : ref ltac:(Self))
+      (_event : multisig.Event.t)
+      : M unit :=
+    let* self : M.Val (ref ltac:(Self)) := M.alloc self in
+    let* _event : M.Val multisig.Event.t := M.alloc _event in
+    let* α0 : ref str.t := M.read (mk_str "not implemented") in
+    let* α1 : never.t := M.call (core.panicking.panic α0) in
+    never_to_any α1.
+  
+  Global Instance AssociatedFunction_emit_event :
+    Notations.DoubleColon ltac:(Self) "emit_event" := {
+    Notations.double_colon := emit_event;
+  }.
+  
+  (*
+      fn transferred_value(&self) -> Balance {
+          unimplemented!()
+      }
+  *)
+  Definition transferred_value
+      (self : ref ltac:(Self))
+      : M ltac:(multisig.Balance) :=
+    let* self : M.Val (ref ltac:(Self)) := M.alloc self in
+    let* α0 : ref str.t := M.read (mk_str "not implemented") in
+    let* α1 : never.t := M.call (core.panicking.panic α0) in
+    never_to_any α1.
+  
+  Global Instance AssociatedFunction_transferred_value :
+    Notations.DoubleColon ltac:(Self) "transferred_value" := {
+    Notations.double_colon := transferred_value;
+  }.
+  
+  (*
+      fn account_id(&self) -> AccountId {
+          unimplemented!()
+      }
+  *)
+  Definition account_id (self : ref ltac:(Self)) : M multisig.AccountId.t :=
+    let* self : M.Val (ref ltac:(Self)) := M.alloc self in
+    let* α0 : ref str.t := M.read (mk_str "not implemented") in
+    let* α1 : never.t := M.call (core.panicking.panic α0) in
+    never_to_any α1.
+  
+  Global Instance AssociatedFunction_account_id :
+    Notations.DoubleColon ltac:(Self) "account_id" := {
+    Notations.double_colon := account_id;
+  }.
+End Impl_multisig_Env_t.
+End Impl_multisig_Env_t.
 
 Module  Multisig.
 Section Multisig.
